src/InputData.dfy
@@ -1,0 +1,9 @@
+class InputData {
+    var weight: real
+    var value: real
+
+    constructor(w: real, v: real) {
+        this.weight := w;
+        this.value := v;
+    }
+}
